Tests.dfy
@@ -14,7 +14,7 @@ module Tests{
         var env := map[];
         var state := map[];
         
-        AnalyzeProgramSound(stmt3, env);
+        AnalyzeProgramSound(stmt3);
         assert AnalyzeStmt(stmt3, state).0;
         match ExecStmt(stmt3, env)
         case Ok(env1) => assert env1["v"] == 4;
@@ -50,7 +50,7 @@ module Tests{
         var env := map[];
         var state := map[];
 
-        AnalyzeProgramSound(stmt, env);
+        AnalyzeProgramSound(stmt);
 
         assert AnalyzeStmt(stmt, state).0;
         
@@ -75,6 +75,8 @@ module Tests{
         var stmt := Seq(if_stmt, Assign("z", Var("x")));
         var env := map[];
         var state := map[];
+
+        AnalyzeProgramSound(stmt);
 
         assert AnalyzeStmt(stmt, state).0;    
         
@@ -146,10 +148,91 @@ module Tests{
         var env := map[];
         var state := map[];
         
-        AnalyzeProgramSound(stmt3, env);
+        AnalyzeProgramSound(stmt3);
         assert AnalyzeStmt(stmt3, state).0;
         match ExecStmt(stmt3, env)
         case Ok(env1) => assert env1["v"] == 0;
+        case Err(e1) => assert false;
+    }
+
+    method TestCaseDivByZero(){
+        /*
+        v := 0;
+        v := 1 / v;
+        */
+        var s1 := Assign("v", Const(0));
+        var s2 := Assign("v", Div(Const(1), Var("v")));
+        var stmt := Seq(s1, s2);
+        var env := map[];
+        var state := map[];
+        
+        var safe := AnalyzeStmt(stmt, state).0;
+        assert !safe;
+        
+        match ExecStmt(stmt, env)
+        case Ok(env1) => assert false;
+        case Err(e1) => assert e1 == DivByZero;
+    }
+
+    method TestCasePruning(){
+        /*
+        if (1) then (x := 5) else (x := 1 / 0);
+        z := x;
+        */
+        var then_stmt := Assign("x", Const(5));
+        var else_stmt := Assign("x", Div(Const(1), Const(0)));
+        var s1 := If(Const(1), then_stmt, else_stmt);
+        var s2 := Assign("z", Var("x"));
+        var stmt := Seq(s1, s2);
+        var env := map[];
+        var state := map[];
+        var safe := AnalyzeStmt(stmt, state).0;
+        assert safe;
+        AnalyzeProgramSound(stmt);
+        match ExecStmt(stmt, env)
+        case Ok(env1) => assert env1["z"] == 5;
+        case Err(e1) => assert false;
+    }
+
+    method TestCaseIncompleteness(){
+        /*
+        z := 2 + (-1);
+        if (z) then (x := 5) else (x := 1 / 0)
+        z := z + x;
+        */
+        var cond := Assign("z", Add(Const(2), Const(-1)));
+        var then_stmt := Assign("x", Const(5));
+        var else_stmt := Assign("x", Div(Const(1), Const(0)));
+        var s1 := If(Var("z"), then_stmt, else_stmt);
+        var s2 := Assign("z", Add(Var("z"), Var("x")));
+        var stmt := Seq(cond, Seq(s1, s2));
+        var env := map[];
+        var state := map[];
+        var safe := AnalyzeStmt(stmt, state).0;
+        assert !safe;
+        match ExecStmt(stmt, env)
+        case Ok(env1) => assert env1["z"] == 6;
+        case Err(e1) => assert false;
+    }
+
+    method TestCaseOverflow(){
+        /*
+        x := 10e17 + (-1);
+        if (x) then (y := 3) else (z := )
+        x := x + y
+        */
+        var cond := Assign("x", Add(Const(1000000000000000000), Const(-1)));
+        var then_stmt := Assign("y", Const(3));
+        var else_stmt := Assign("z", Const(2));
+        var s1 := If(Var("x"), then_stmt, else_stmt);
+        var s2 := Assign("x", Add(Var("x"), Var("y")));
+        var stmt := Seq(cond, Seq(s1, s2));
+        var env := map[];
+        var state := map[];
+        var safe := AnalyzeStmt(stmt, state).0;
+        assert !safe;
+        match ExecStmt(stmt, env)
+        case Ok(env1) => assert env1["x"] == 1000000000000000002;
         case Err(e1) => assert false;
     }
 }
